src/Layer1to2RefinementDefinitions.v
@@ -49,14 +49,15 @@ Fixpoint oracle_refines_to T (d1: State layer1_lts) (p: Layer2.prog T)  (o1: Ora
     | @Bind T1 T2 p1 p2 =>
       exists o1' o1'',
       o1 = o1'++o1'' /\
-      (forall d1', Layer1Definitions.exec o1 d1 (compile p1) (Crashed d1') ->
-         oracle_refines_to T1 d1 p1 o1 o2 /\ o1'' = []) /\
-      (forall d1' r,
-         Layer1Definitions.exec o1' d1 (compile p1) (Finished d1' r) ->
+     ((exists d1', Layer1Definitions.exec o1 d1 (compile p1) (Crashed d1') /\
+         oracle_refines_to T1 d1 p1 o1 o2 /\ o1'' = []) \/
+      (exists d1' r ret,
+          Layer1Definitions.exec o1' d1 (compile p1) (Finished d1' r) /\
+          Layer1Definitions.exec o1'' d1' (compile (p2 r)) ret /\
          exists o2' o2'',
          oracle_refines_to T1 d1 p1 o1' o2' /\
          oracle_refines_to T2 d1' (p2 r) o1'' o2'' /\
-         o2 = o2' ++ o2'')
+         o2 = o2' ++ o2''))
     | Read _ =>
       if (in_dec Layer1Definitions.token_dec Layer1Definitions.Crash o1) then
         o2 = [Crash1]
