src/Layer2Facts.v
@@ -1,0 +1,32 @@
+Require Import Primitives Simulation Layer2Definitions.
+
+Lemma layer2_finished_not_crashed_oracle_app:
+  forall T (p: prog T) o1 o2 s s1 s2 r1,
+    exec o1 s p (Finished s1 r1) ->
+    ~exec (o1++o2) s p (Crashed s2).
+Proof.
+  unfold not; induction p; simpl; intros;
+    repeat match goal with
+           | [H: exec _ _ _ _ |- _] =>
+             inversion H; sigT_eq; cleanup; clear H
+           end; simpl; eauto.
+  simpl in *; cleanup.
+  rewrite <- app_assoc in H2.
+  -
+    admit.
+  - rewrite <- app_assoc in H6; eauto.
+Admitted.
+
+Lemma layer2_finished_oracle_length_eq:
+  forall T (p: prog T) o1 o2 s s1 s2 r1 r2,
+      exec o1 s p (Finished s1 r1) ->
+      exec o2 s p (Finished s2 r2) ->
+      length o1 = length o2.
+Proof.
+  induction p; intros;
+    repeat match goal with
+           | [H: exec _ _ _ _ |- _] =>
+             inversion H; sigT_eq; cleanup; clear H
+           end; simpl; eauto.
+  repeat rewrite app_length.
+  specialize IHp with (1:= H6)(2:= H7); cleanup.
